Improve inline algorithm.

theories/inline/compile.v
@@ -8,83 +8,96 @@ Implicit Types prog : data_program.
 Definition inline_annotation :=
   "inline".
 
-Fixpoint inline_compile_expr prog e :=
+Definition inline_max_depth :=
+  10.
+
+Fixpoint inline_compile_expr prog depth := fix inline_compile_expr' e :=
   match e with
   | DataVal _
   | DataVar _ =>
       e
   | DataLet e1 e2 =>
       DataLet
-        (inline_compile_expr prog e1)
-        (inline_compile_expr prog e2)
+        (inline_compile_expr' e1)
+        (inline_compile_expr' e2)
   | DataCall e1 e2 =>
       match e1 with
       | DataVal (DataFunc func annot) =>
           match bool_decide (inline_annotation ∈ annot), prog !! func with
           | true, Some e_func =>
+              let e_func :=
+                match depth with
+                | 0 =>
+                    e_func
+                | S depth =>
+                    inline_compile_expr prog depth e_func
+                end
+              in
               DataLet
-                (inline_compile_expr prog e2)
+                (inline_compile_expr' e2)
                 e_func
           | _, _ =>
               DataCall
-                (inline_compile_expr prog e1)
-                (inline_compile_expr prog e2)
+                (inline_compile_expr' e1)
+                (inline_compile_expr' e2)
           end
       | _ =>
           DataCall
-            (inline_compile_expr prog e1)
-            (inline_compile_expr prog e2)
+            (inline_compile_expr' e1)
+            (inline_compile_expr' e2)
       end
   | DataUnop op e =>
       DataUnop op
-        (inline_compile_expr prog e)
+        (inline_compile_expr' e)
   | DataBinop op e1 e2 =>
       DataBinop op
-        (inline_compile_expr prog e1)
-        (inline_compile_expr prog e2)
+        (inline_compile_expr' e1)
+        (inline_compile_expr' e2)
   | DataBinopDet op e1 e2 =>
       DataBinopDet op
-        (inline_compile_expr prog e1)
-        (inline_compile_expr prog e2)
+        (inline_compile_expr' e1)
+        (inline_compile_expr' e2)
   | DataIf e0 e1 e2 =>
       DataIf
-        (inline_compile_expr prog e0)
-        (inline_compile_expr prog e1)
-        (inline_compile_expr prog e2)
+        (inline_compile_expr' e0)
+        (inline_compile_expr' e1)
+        (inline_compile_expr' e2)
   | DataConstr tag e1 e2 =>
       DataConstr tag
-        (inline_compile_expr prog e1)
-        (inline_compile_expr prog e2)
+        (inline_compile_expr' e1)
+        (inline_compile_expr' e2)
   | DataConstrDet tag e1 e2 =>
       DataConstrDet tag
-        (inline_compile_expr prog e1)
-        (inline_compile_expr prog e2)
+        (inline_compile_expr' e1)
+        (inline_compile_expr' e2)
   | DataLoad e1 e2 =>
       DataLoad
-        (inline_compile_expr prog e1)
-        (inline_compile_expr prog e2)
+        (inline_compile_expr' e1)
+        (inline_compile_expr' e2)
   | DataStore e1 e2 e3 =>
       DataStore
-        (inline_compile_expr prog e1)
-        (inline_compile_expr prog e2)
-        (inline_compile_expr prog e3)
+        (inline_compile_expr' e1)
+        (inline_compile_expr' e2)
+        (inline_compile_expr' e3)
   end.
+#[global] Arguments inline_compile_expr _ _ !_ / : assert.
 
 Definition inline_compile prog :=
-  (inline_compile_expr prog) <$> prog.
+  (inline_compile_expr prog inline_max_depth) <$> prog.
 
-Lemma inline_compile_expr_sound prog e :
-  inline_expr prog e (inline_compile_expr prog e).
+Lemma inline_compile_expr_sound prog depth e :
+  inline_expr prog e (inline_compile_expr prog depth e).
 Proof.
-  induction e; eauto with inline.
-  do 4 (simpl; case_match; eauto with inline).
+  revert e. induction depth; induction e.
+  all: eauto with inline.
+  all: do 4 (simpl; case_match; eauto with inline).
 Qed.
 Lemma inline_compile_sound prog :
   inline prog (inline_compile prog).
 Proof.
   split.
   - rewrite dom_fmap_L //.
-  - intros func e Hfunc. exists (inline_compile_expr prog e). split.
+  - intros func e Hfunc. eexists. split.
     + apply inline_compile_expr_sound.
     + rewrite lookup_fmap Hfunc //.
 Qed.
